Remove axioms for Tok definition.

src/program_logic/crash_inv.v
@@ -1,4 +1,5 @@
 From iris.proofmode Require Import base tactics classes.
+From iris.algebra Require Import excl.
 From iris.base_logic Require Export invariants.
 From iris.program_logic Require Export weakestpre.
 From Perennial.program_logic Require Import staged_invariant crash_weakestpre.
@@ -8,31 +9,35 @@ Import uPred.
 Section ci.
 Context `{!irisG Λ Σ}.
 Context `{!stagedG Σ}.
+Context `{inG Σ (exclR unitO)}.
 
-Axiom Tok: iProp Σ.
-Axiom Tok_Tok : Tok ∗ Tok -∗ False.
-Instance timeless_Tok: Timeless (Tok).
-Admitted.
+Definition Tok (γ: gname) :=
+  own γ (Excl ()).
 
+Lemma Tok_Tok γ: Tok γ ∗ Tok γ -∗ False.
+Proof. iIntros "(H1&H2)". by iDestruct (own_valid_2 with "H1 H2") as %?. Qed.
 
-Definition detached_staged k E1 E2 P : iProp Σ :=
+Instance timeless_Tok γ: Timeless (Tok γ).
+Proof. rewrite /Tok. apply _. Qed.
+
+Definition ci_staged k E1 E2 P : iProp Σ :=
   (|={E1, ∅}=> |={∅, ∅}▷=>^k |={∅, E2}=> P)%I.
 
-Definition detached_ci k E1 E2 N (P: iProp Σ) : iProp Σ :=
-  P ∨ (∃ γ, Tok ∗ staged_inv N γ (detached_staged k E1 E2 P))%I.
+Definition ci_inv_inner k E1 E2 N (P: iProp Σ) γ : iProp Σ :=
+  P ∨ (∃ γ', Tok γ ∗ staged_inv N γ' (ci_staged k E1 E2 P))%I.
 
-Lemma wpc_staged_invariant_aux s k E1 E2 E1' E2' e Φ Φc P Q1 R1 Q2 R2 N1 N2 γ :
+Lemma wpc_staged_invariant_aux s k E1 E2 E1' E2' e Φ Φc P Q1 R1 Q2 R2 N1 N2 γ γ' :
   ↑N1 ⊆ E1 →
   ↑N2 ⊆ E1 →
   (E2' ⊆ E1') →
   (E1 ⊆ E1') →
   (E2' ⊆ E2) →
   N1 ## N2 →
-  inv N1 (detached_ci (2 * S (S (S k))) E1' E2' N2 P) ∗
+  inv N1 (ci_inv_inner (2 * S (S (S k))) E1' E2' N2 P γ) ∗
   □ (Q1 -∗ R1) ∗
   □ (Q2 -∗ R2) ∗
-  staged_inv N2 γ (detached_staged (2 * (S (S (S k)))) E1' E2' P) ∗
-  staged_value N2 γ (|={E1 ∖ ↑N1 ∖ ↑N2, ∅}=> |={∅, ∅}▷=>^(S k)
+  staged_inv N2 γ' (ci_staged (2 * (S (S (S k)))) E1' E2' P) ∗
+  staged_value N2 γ' (|={E1 ∖ ↑N1 ∖ ↑N2, ∅}=> |={∅, ∅}▷=>^(S k)
                      |={∅, E1 ∖ ↑N1 ∖ ↑N2}=>
                      Q1 ∗ WPC e @ k; E1 ∖ ↑N1 ∖ ↑N2;E2 {{ v, (Φ v ∧ |={E1,E2}=> Φc) ∗ P }}{{Φc ∗ P}} ∗ Q2) ⊢
   |={E1, ∅}=> |={∅, ∅}▷=>^(S (S (S k))) |={∅, E1}=> R1 ∗ WPC e @ s; S (S k); E1; E2 {{ v, Φ v }} {{Φc}} ∗ R2.
@@ -62,7 +67,7 @@ Proof.
     iMod "Hclo".
     iMod ("Hclo'" with "[HP]").
     { iSplitL. iApply "HP". iAlways.
-      iIntros. rewrite /detached_staged.
+      iIntros. rewrite /ci_staged.
       iApply step_fupdN_inner_later; first auto.
       iNext. eauto.
     }
@@ -72,7 +77,7 @@ Proof.
     iSplitR "HQ2"; last first.
     { by iApply "HQR2". }
     iSplit.
-    - by iDestruct "HΦ" as "($&_)".
+    - iDestruct "HΦ" as "($&_)". eauto.
     - iDestruct "HΦ" as "(_&HΦ)".
       iMod "HΦ". iMod (fupd_intro_mask' _ ∅) as "?"; first by set_solver.
       iModIntro.
@@ -100,7 +105,7 @@ Proof.
     iIntros "H".
     rewrite wpc_unfold /wpc_pre.
     rewrite Hval. iDestruct "H" as "(_&HP)".
-    rewrite /detached_staged.
+    rewrite /ci_staged.
     iMod (fupd_intro_mask') as "Hclo"; [| iMod "HP"].
     { set_solver. }
     iModIntro.
@@ -153,7 +158,7 @@ Proof.
     iSpecialize ("Hclo'" $! _ with "[H]").
     { iSplitL "H". iApply "H".
       iAlways. iIntros "H".
-      rewrite /detached_staged.
+      rewrite /ci_staged.
       replace (2 * S (S (S k))) with (S (S (S k)) + S (S (S k))) by lia.
       iApply step_fupdN_inner_plus.
       iMod (fupd_intro_mask' _ (E1 ∖ ↑N1 ∖ ↑N2)) as "Hclo''".
@@ -204,29 +209,29 @@ Proof.
     eauto.
 Qed.
 
-Lemma detached_ci_tok k E1 E2 N P:
-  ▷ detached_ci k E1 E2 N P -∗
-  Tok -∗
-  ▷ (P ∗ Tok).
+Lemma detached_ci_tok k E1 E2 N P γ:
+  ▷ ci_inv_inner k E1 E2 N P γ -∗
+  Tok γ -∗
+  ▷ (P ∗ Tok γ).
 Proof.
   iIntros "HCI HTok".
   iNext.
-  rewrite /detached_ci.
+  rewrite /ci_inv_inner.
   iDestruct "HCI" as "[$|H]".
   - iFrame.
   - iDestruct "H" as (?) "(H&?)".
     iDestruct (Tok_Tok with "[$]") as "[]".
 Qed.
 
-Lemma wpc_staged_invariant s k E1 E2 E1' E2' e Φ Φc P N1 N2 :
+Lemma wpc_staged_invariant s k E1 E2 E1' E2' e Φ Φc P N1 N2 γ :
   ↑N1 ⊆ E1 →
   ↑N2 ⊆ E1 →
   (E2' ⊆ E1') →
   (E1 ⊆ E1') →
   (E2' ⊆ E2) →
   N1 ## N2 →
-  inv N1 (detached_ci (2 * S (S (S k))) E1' E2' N2 P) ∗
-  Tok ∗
+  inv N1 (ci_inv_inner (2 * S (S (S k))) E1' E2' N2 P γ) ∗
+  Tok γ ∗
   (▷ (P) -∗ WPC e @ NotStuck; k; (E1 ∖ ↑N1 ∖ ↑N2); E2
                 {{ λ v, (Φ v ∧ |={E1,E2}=> Φc) ∗ P}} {{ Φc ∗ P }}) ⊢
   WPC e @ s; (S (S k)); E1; E2 {{ Φ }} {{ Φc }}.
@@ -293,7 +298,7 @@ Proof.
     iIntros "Hwp".
     iMod (staged_inv_alloc N2 _
              (|={E1', ∅}=> |={∅, ∅}▷=>^(2 * S (S (S k))) |={∅, E2'}=>P)%I _ with "[Hwp]")
-      as (γ) "(#Hsi&Hval)".
+      as (γ') "(#Hsi&Hval)".
     { iSplitL "Hwp". iApply "Hwp".
        iAlways. iIntros "(_&Hwp)".
        iMod (fupd_intro_mask' _ ∅) as "Hclo"; first by set_solver+.
@@ -348,7 +353,7 @@ Proof.
       iMod "Hclo'".
       iApply fupd_mask_weaken; auto.
     }
-    iAssert (|={E1 ∖ ↑N1 ∖ ↑N2,E1 ∖ ↑N1}=> staged_value N2 γ _)%I with "[Hclo']" as "H".
+    iAssert (|={E1 ∖ ↑N1 ∖ ↑N2,E1 ∖ ↑N1}=> staged_value N2 γ' _)%I with "[Hclo']" as "H".
     {
     iApply fupd_mask_frame.
     2: { iMod "Hclo'". iModIntro.
@@ -368,7 +373,7 @@ Proof.
     iApply (wpc_staged_invariant_aux s k E1 E2 E1' E2'
                   _ Φ Φc P
                   (state_interp σ2 a1 (strings.length efs + a2)) _
-                  ([∗ list] ef ∈ efs, WPC ef @ k; ⊤;∅ {{ v, fork_post v }}{{True}})%I  _ N1 N2 with "[H]"); try assumption.
+                  ([∗ list] ef ∈ efs, WPC ef @ k; ⊤;∅ {{ v, fork_post v }}{{True}})%I  _ N1 N2 γ with "[H]"); try assumption.
     { iIntros. iFrame "Hinv". iFrame "H".
       iFrame "Hsi". iSplit.
       - eauto.
